rearrange Coq directory structure and file contents

src/OpalInterp.v
@@ -1,909 +1,210 @@
-Require Import OpalSrc.OpalSemantics OpalSrc.OpalUtil CpdtTactics.
+Require Import Opal.OpalSemantics CpdtTactics.
 
 
-Definition empty_env : var_store := StringPairMap.empty sexp_value.
+Fixpoint eval_eq (l r: sexp) {lp: sexp_is_value l} {rp: sexp_is_value r}
+  : bool_value.
+  unshelve
+    refine (
+      match l as l', r as r'
+            return l=l' -> r=r' -> bool_value
+      with
+      | EmptySexp, EmptySexp =>
+        fun _ _ =>
+          exist _ TrueBool _
+      | (ConsSexp ll lr), (ConsSexp rl rr) =>
+        fun _ _ =>
+          let leqv := eval_eq ll rl _ _ in
+          let leq := proj1_sig leqv in
+          let reqv := eval_eq lr rr _ _ in
+          let req := proj1_sig reqv in
+          match leq as leq', req as req'
+                return leq=leq' -> req=req' -> bool_value
+          with
+          | TrueBool, TrueBool =>
+            fun _ _ =>
+              exist _ TrueBool _
+          | _, _ =>
+            fun _ _ =>
+              exist _ FalseBool _
+          end eq_refl eq_refl
+      | _, _ =>
+        fun _ _ =>
+          exist _ FalseBool _
+      end eq_refl eq_refl) ;
+    auto ;
+    subst ;
+    inversion lp ;
+    inversion rp ;
+    eauto.
+Defined.
 
-Definition set_env (e: var_store) (n: node) (v: var) (val: sexp_value) : var_store :=
-  StringPairMap.add (n, v) val e.
+Arguments eval_eq l r : clear implicits.
 
-Definition get_env (e: var_store) (n: node) (v: var) : option sexp_value :=
-  StringPairMap.find (n, v) e.
+Fixpoint eval_mem
+         (l r: sexp) {lp: sexp_is_value l} {rp: sexp_is_value r}
+  : bool_value.
+  unshelve
+    refine (
+      match r as r' return r=r' -> bool_value with
+      | EmptySexp => fun _ => exist _ FalseBool _
+      | ConsSexp rl rr =>
+        fun _ =>
+          let eqv := eval_eq l rl _ _ in
+          let eq := proj1_sig eqv in
+          match eq as eq' return eq=eq' -> bool_value with
+          | TrueBool =>
+            fun _ => exist _ TrueBool _
+          | FalseBool =>
+            fun _ => eval_mem l rr lp _
+          | _ =>
+            fun _ => _
+          end eq_refl
+      | _ => fun _ => exist _ FalseBool _
+      end eq_refl
+    ) ;
+    subst ;
+    eauto ;
+    inversion rp ;
+    eauto.
+Defined.
 
-Fixpoint lookup (n: node) (v: var) (Sigma: var_store_stack)
-  : (sexp_value + error) :=
-  match Sigma with
-  | nil => inr (LookupErr n v)
-  | cons e rest =>
-    match get_env e n v with
-    | Some res => inl res
-    | None => lookup n v rest
-    end
-  end.
+Arguments eval_mem l r : clear implicits.
 
-Definition empty_world_store : world_store :=
-  fun _ => None.
-
-Definition set_world_store (w: world_store) (u: world) (S: var_store_stack) (s: var_store) : world_store :=
-  fun u' =>
-    match string_dec u u' with
-    | left _ => Some (S, s)
-    | right _ => w u'
-    end.
-
-Definition empty_handlers : handlers :=
-  fun _ => None.
-
-Definition set_handler (h: handlers) (o: op) (n: node) (v: var) (s: sexp) : handlers :=
-  fun o' =>
-    match string_dec o o' with
-    | left _ => Some (n, v, s)
-    | right _ => h o'
-    end.
-
-Definition empty_mergers : mergers :=
-  fun _ _ => None.
-
-Definition set_merger (m: mergers) (n: node) (v: var) (s: sexp) : mergers :=
-  fun n' v' =>
-    match (string_dec n n', string_dec v v') with
-    | (left _, left _) => Some s
-    | _ => m n' v'
-    end.
-
-Fixpoint sexp_step (s: sexp) (Sigma: var_store_stack) (pi: principals)
-  : (sexp_value + error) :=
-  match s with
-  | EmptySet => inl (exist sexp_is_value EmptySet EmptySetIsValue)
-  | Cons l r =>
-    match (sexp_step l Sigma pi), (sexp_step r Sigma pi) with
-    | inl (exist _ lv Hl), inl (exist _ rv Hr) =>
-      inl (exist _ (Cons lv rv) (ConsValuesIsValue Hl Hr))
-    | inr err, _ => inr err
-    | _, inr err => inr err
-    end
-  | Var n v =>
-    match set_mem string_dec n pi with
-    | true => lookup n v Sigma
-    | false => inr (ReadPermErr n v pi)
-    end
-  end.
-
-Lemma canonical_sexp_value :
-  forall v Sigma pi H,
-    sexp_step v Sigma pi = inl (exist sexp_is_value v H).
-Proof.
-  induction v ; intros.
-  * specialize proof_irrelevance with (sexp_is_value EmptySet) EmptySetIsValue H.
-    crush.
-  * inversion H.
-  * inversion H.
-    specialize IHv1 with Sigma pi H2.
-    specialize IHv2 with Sigma pi H3.
-    specialize proof_irrelevance with (sexp_is_value (Cons v1 v2))
-                                      (ConsValuesIsValue H2 H3) H.
-    crush.
-Qed.
-
-Lemma canonical_sexp_cons :
-  forall v l r Sigma pi H,
-  sexp_is_value v ->
-  sexp_step v Sigma pi = inl (exist sexp_is_value (Cons l r) H) ->
-  v = (Cons l r).
-Proof.
-  intros.
-  induction v.
-  * unfold sexp_step in H0.
-    fold sexp_step in H0.
-    destruct (sexp_step l Sigma pi).
-  - destruct s.
-    destruct (sexp_step r Sigma pi).
-    + destruct s0. crush.
-    + discriminate.
-  - discriminate.
-  * inversion H0.
-  * inversion H0.
-    specialize canonical_sexp_value with v1 Sigma pi H4.
-    specialize canonical_sexp_value with v2 Sigma pi H5.
-    intros.
-    subst.
-    unfold sexp_step in H1.
-    fold sexp_step in H1.
-    destruct (sexp_step v1 Sigma pi) ;
-      destruct (sexp_step v2 Sigma pi) ;
-      try (destruct s;
-           destruct s0);
-      crush.
-Qed.
-
-
-
-Lemma canonical_sexp_value_2 :
-  forall v v' Sigma pi H,
-    sexp_is_value v ->
-    sexp_step v Sigma pi = inl (exist sexp_is_value v' H) ->
-    v = v'.
-Proof.
-  induction v ; intros.
-  * crush.
-  * inversion H0.
-  * inversion H0.
-    subst.
-    inversion H1.
-    destruct (sexp_step v1 Sigma pi) eqn:?.
-    - destruct s.
-      destruct (sexp_step v2 Sigma pi) eqn:?.
-      + destruct s0.
-        specialize IHv1 with x Sigma pi s.
-        specialize IHv2 with x0 Sigma pi s0.
-        crush.
-      + crush.
-    - crush.
-Qed.
-
-Inductive bool_lt : bool -> bool -> Prop :=
-| ValueLt : forall b1 b2,
-    bool_is_value b1 ->
-    ~ bool_is_value b2 ->
-    bool_lt b1 b2
-| SexpValueLtEqL : forall s1 s2 s3,
-    sexp_is_value s1 ->
-    ~sexp_is_value s2 ->
-    bool_lt (Eq s1 s3) (Eq s2 s3)
-| SexpValueLtEqR : forall s1 s2 s3,
-    sexp_is_value s1 ->
-    ~sexp_is_value s2 ->
-    bool_lt (Eq s3 s1) (Eq s3 s2)
-| SexpValueLtMemL : forall s1 s2 s3,
-    sexp_is_value s1 ->
-    ~sexp_is_value s2 ->
-    bool_lt (Mem s1 s3) (Mem s2 s3)
-| SexpValueLtMemR : forall s1 s2 s3,
-    sexp_is_value s1 ->
-    ~sexp_is_value s2 ->
-    bool_lt (Mem s3 s1) (Mem s3 s2)
-| ConjLtL : forall b1 b2,
-    bool_lt b1 (Conj b1 b2)
-| ConjLtR : forall b1 b2,
-    bool_lt b2 (Conj b1 b2)
-| DisjLtL : forall b1 b2,
-    bool_lt b1 (Disj b1 b2)
-| DisjLtR : forall b1 b2,
-    bool_lt b2 (Disj b1 b2)
-| EqLt : forall ll lr rl rr,
-    sexp_is_value ll ->
-    sexp_is_value lr ->
-    sexp_is_value rl ->
-    sexp_is_value rr ->
-    bool_lt (Conj (Eq ll rl) (Eq lr rr)) (Eq (Cons ll lr) (Cons rl rr))
-| MemLt : forall l rl rr,
-    sexp_is_value l ->
-    sexp_is_value rl ->
-    sexp_is_value rr ->
-    bool_lt (Disj (Eq l rl) (Mem l rr)) (Mem l (Cons rl rr))
-.
-
-Lemma acc_true : Acc bool_lt True.
-Proof.
-  constructor ;
-  intros ;
-  inversion H ;
-  contradiction H1 ;
-  constructor.
-Qed.
-
-Lemma acc_false : Acc bool_lt False.
-Proof.
-  constructor ;
-  intros ;
-  inversion H ;
-  contradiction H1 ;
-  constructor.
-Qed.
-
-Lemma acc_eq_val : forall s1 s2,
-    sexp_is_value s1 ->
-    sexp_is_value s2 ->
-    Acc bool_lt (Eq s1 s2).
-Proof.
-  Hint Constructors bool_is_value sexp_is_value.
-  Hint Resolve acc_true acc_false.
-  Ltac DKill y H1 H2 H3 H4 :=
-    constructor ;
-    intros ;
-    destruct y ;
-    inversion H1 ;
-    inversion H2 ;
-    inversion H3 ;
-    try (solve [contradiction H4]) ;
-    auto.
-
-  induction s1 ; induction s2 ; intros ;
-    try (solve [ DKill y H H1 H2 H7
-               | inversion H ;
-                 DKill y H5 H5 H6 H11
-        ]).
-  * intros.
-    inversion H.
-    inversion H0.
-    specialize (IHs1_1 s2_1 H3 H7).
-    specialize (IHs1_2 s2_2 H4 H8).
-    constructor.
-    intros.
-    destruct y ; inversion H9;
-      try (solve [inversion H10]) ;
-      try (solve [contradiction H15]) ;
-      auto.
-    subst.
-    constructor.
-    intros.
-    destruct y ; inversion H1;
-      try (solve [inversion H2]) ; auto.
-Qed.
-
-Lemma acc_eq : forall s1 s2, Acc bool_lt (Eq s1 s2).
-Proof.
-  Hint Constructors bool_is_value sexp_is_value.
-  Hint Resolve acc_true acc_false acc_eq_val.
-  induction s1 ; induction s2 ; auto.
-  * constructor ; intros. destruct y ; inversion H ;
-      try (solve [inversion H0]) ;
-      try (solve [contradiction H5 ; constructor]);
-      auto.
-  * constructor ; intros. destruct y ; inversion H ;
-      try (solve [inversion H0]) ;
-      try (solve [contradiction H5 ; constructor]);
-      auto.
-  * constructor ; intros. destruct y ; inversion H ;
-      try (solve [inversion H0]) ;
-      try (solve [contradiction H5 ; constructor]);
-      auto.
-  * constructor ; intros. destruct y ; inversion H.
-    - inversion H0.
-    - destruct s ; inversion H.
-      + inversion H6.
-      + subst.
-        inversion H.
-        ** inversion H0.
-        ** subst.
-           constructor.
-           intros.
-           destruct y ; inversion H0;
-             auto ;
-             inversion H1;
-             contradiction H13.
-      + inversion H6.
-      + inversion H9.
-      + subst. inversion H9.
-      + inversion H6.
-      + subst.
-        inversion H.
-        ** inversion H0.
-        ** subst.
-           constructor.
-           intros.
-           destruct y ; inversion H0;
-             auto ;
-             inversion H1;
-             contradiction H13.
-    - subst.
-      destruct s0 ; inversion H.
-      + inversion H0.
-      + constructor.
-        intros.
-        destruct y ; inversion H7;
-          auto;
-          inversion H8 ;
-          contradiction H13.
-      + inversion H0.
-      + inversion H4.
-      + inversion H4.
-      + inversion H0.
-      + constructor.
-        intros.
-        destruct y ; inversion H7;
-          auto;
-          inversion H8 ;
-          contradiction H13.
-    - inversion H0.
-    - inversion H0.
-    - inversion H0.
-    - auto.
-    - auto.
-
-  * constructor ; intros. destruct y ; inversion H.
-    - inversion H0.
-    - destruct s ; inversion H.
-      + inversion H6.
-      + subst.
-        inversion H.
-        ** inversion H0.
-        ** subst.
-           constructor.
-           intros.
-           destruct y ; inversion H0;
-             auto ;
-             inversion H1;
-             contradiction H13.
-      + inversion H6.
-      + inversion H9.
-      + inversion H3.
-      + inversion H6.
-      + subst.
-        inversion H.
-        ** inversion H0.
-        ** subst.
-           constructor.
-           intros.
-           destruct y ; inversion H0 ; auto.
-           -- inversion H1.
-           -- contradiction H13.
-           -- inversion H1.
-           -- inversion H1.
-           -- subst.
-              constructor.
-              intros.
-              destruct y ; inversion H1 ; auto ; try (inversion H2).
-           -- inversion H1.
-    - subst.
-      constructor.
-      intros.
-      destruct y ; inversion H0 ; inversion H1; auto. contradiction H8.
-    - inversion H0.
-    - inversion H0.
-    - inversion H0.
-    - auto.
-    - auto.
- * subst.
-   constructor.
-   intros.
-   destruct y ; inversion H ; auto; inversion H0 ; contradiction H5; auto.
- * constructor.
-   intros.
-   destruct y ; inversion H ;auto; inversion H0 ; try (solve [contradiction H5]); auto.
-   - subst.
-constructor.
-   intros.
-   destruct y ; inversion H0 ; auto; inversion H1. contradiction H9.
-   - subst.
-     constructor.
-     intros.
-     destruct y ; inversion H0 ; auto; inversion H1. contradiction H9.
-     subst.
-     constructor.
-     intros.
-     destruct y ; inversion H1; auto ; inversion H2.
-  *
-    constructor.
-    intros.
-    destruct y ; inversion H ; auto ; inversion H0.
-   - subst.
-     constructor. intros.
-     destruct y ; inversion H0 ; auto ; inversion H1. contradiction H9.
-     subst.
-     constructor. intros.
-     destruct y ; inversion H1 ; auto ; inversion H2.
-   - subst.
-     constructor. intros.
-     destruct y ; inversion H0 ; auto ; inversion H1. contradiction H9.
-     subst.
-     constructor. intros.
-     destruct y ; inversion H1 ; auto ; inversion H2.
-   - subst.
-     constructor. intros.
-     destruct y ; inversion H0 ; auto ; inversion H1.
-Qed.
-
-Lemma acc_mem_val : forall s1 s2,
-    sexp_is_value s1 ->
-    sexp_is_value s2 ->
-    Acc bool_lt (Mem s1 s2).
-Proof.
-  Hint Constructors bool_is_value sexp_is_value.
-  Hint Resolve acc_true acc_false.
-  induction s2 ; intros ;
-    try (solve [ DKill y H H1 H2 H7
-               | inversion H ;
-                 DKill y H5 H5 H6 H11
-        ]).
-  * constructor.
-    intros.
-    destruct y ; inversion H1; auto ; inversion H2.
-    - constructor.
-      intros.
-      destruct y ; inversion H0; auto.
-      + subst.
-        inversion H9. inversion H2.
-      + inversion H9.
-        ** subst. inversion H10.
-        ** subst. contradiction H15.
-        ** subst. contradiction H15.
-      + inversion H9.
-        ** subst. inversion H10.
-      + inversion H9.
-        ** subst. inversion H10.
-    -contradiction H7.
-  * inversion H0.
-  * constructor.
-    intros.
-    destruct y ; inversion H1; auto; inversion H2 ; try (solve [contradiction H7]).
-    subst.
-    constructor.
-    intros.
-    destruct y ; inversion H2; auto ; inversion H3 ; try (solve [contradiction H7]).
-Qed.
-
-Lemma acc_mem : forall s2 s1, Acc bool_lt (Mem s1 s2).
-Proof.
-  Hint Constructors bool_is_value sexp_is_value.
-  Hint Resolve acc_true acc_false acc_eq_val acc_eq acc_mem_val.
-  induction s2; intros.
-  * constructor. intros.
-    destruct y ; inversion H; auto ; inversion H0. contradiction H5. auto.
-  * constructor. intros.
-    destruct y ; inversion H; auto ; inversion H0.
-  - constructor. intros.
-    destruct y ; inversion H7; auto ; inversion H8. contradiction H13.
-  - constructor. intros.
-    destruct y ; inversion H7; auto ; inversion H8. contradiction H13.
-    subst.
-    constructor. intros.
-    destruct y ; inversion H0; auto ; inversion H1.
-  * constructor.
-    intros.
-    destruct y ; inversion H; auto ; inversion H0 ; subst.
-    - constructor.
-      intros.
-      destruct y ; inversion H0 ; auto ; inversion H1. contradiction H9.
-      subst.
-      constructor.
-      intros.
-      destruct y ; inversion H1 ; auto ; inversion H2.
-    - constructor.
-      intros.
-      destruct y ; inversion H0 ; auto ; inversion H1. contradiction H9.
-      constructor.
-      intros.
-      destruct y ; inversion H12 ; auto ; inversion H13.
-    - constructor.
-      intros.
-      destruct y ; inversion H0 ; auto ; inversion H1.
-Qed.
-
-Lemma acc_all : forall b, Acc bool_lt b.
-Proof.
-  Hint Constructors bool_is_value sexp_is_value.
-  Hint Resolve acc_true acc_false acc_eq acc_mem.
-  Ltac foobar y H1 H2 := constructor ; intros ; destruct y ; inversion H1 ; auto ; inversion H2.
-  induction b ; try (solve [foobar y H H0]).
-  * apply acc_eq.
-  * apply acc_mem.
-  * constructor.
-    intros.
-    destruct y ; inversion H; subst; auto ; try (solve [inversion H0]).
-  * constructor.
-    intros.
-    destruct y ; inversion H; subst; auto ; try (solve [inversion H0]).
-Qed.
-
-Lemma bool_lt_wf : well_founded bool_lt.
-Proof.
-  unfold well_founded.
-  apply acc_all.
-Qed.
-
-Require Import Relation_Operators.
-
-Lemma rel_trans : forall A (R: A -> A -> Prop),
-    well_founded R -> well_founded (clos_trans A R).
-Proof.
-  intros.
-  unfold well_founded.
-  unfold well_founded in H.
-  specialize Acc_inv. intros.
-  specialize (H0 A R).
-  intros.
-  induction (H a).
-  * constructor.
-    intros.
-    induction H3.
-    - auto.
-    - intuition.
-      eapply IHclos_trans1; auto.
-      intros.
-      specialize (Acc_inv H4).
-      crush.
-Qed.
-
-Definition bool_lt_trans := clos_trans bool bool_lt.
-Definition bool_lt_trans_wf : well_founded bool_lt_trans := rel_trans bool_lt_wf.
-
-
-Definition bool_step : forall (Sigma: var_store_stack)
-                              (pi: principals),
-    bool -> (bool_value + error).
-  intros Sigma pi.
-  refine (
-      Fix bool_lt_trans_wf
-          (fun _ => (sum bool_value error))
-          (fun (b: bool)
-               (bool_step : forall y : bool, bool_lt_trans y b -> (bool_value + error)) =>
-             match b as b' return b = b' -> (bool_value + error) with
-             | True => fun _ => inl (exist _ True TrueIsValue)
-             | False => fun _ => inl (exist _ False FalseIsValue)
-             | Conj l r =>
-               fun _ =>
-                 match bool_step l _ as linner, bool_step r _ as rinner
-                       return (bool_step l _) = linner ->
-                              (bool_step r _) = rinner ->
-                              (bool_value + error)
-                 with
-                 | inl lv, inl rv =>
-                   fun _ _ =>
-                     match (proj1_sig lv) as lv', (proj1_sig rv) as rv'
-                           return (proj1_sig lv)=lv' ->
-                                  (proj1_sig rv)=rv' ->
-                                  (bool_value + error)
-                     with
-                     | True, True =>
-                       fun _ _ => inl (exist _ True _)
-                     | False, _ =>
-                       fun _ _ => inl (exist _ False _)
-                     | _, False =>
-                       fun _ _ => inl (exist _ False _)
-                     | _, _ =>
-                       fun _ _ => inr (BoolEvalErr b)
-                     end eq_refl eq_refl
-                 | inr err, _ =>
-                   fun _ _ => inr err
-                 | _, inr err =>
-                   fun _ _ => inr err
-                 end eq_refl eq_refl
-             | Disj l r =>
-               fun _ =>
-                 match bool_step l _ as linner, bool_step r _ as rinner
-                       return (bool_step l _) = linner ->
-                              (bool_step r _) = rinner ->
-                              (bool_value + error)
-                 with
-                 | inl lv, inl rv =>
-                   fun _ _ =>
-                     match (proj1_sig lv) as lv', (proj1_sig rv) as rv'
-                           return (proj1_sig lv)=lv' ->
-                                  (proj1_sig rv)=rv' ->
-                                  (bool_value + error)
-                     with
-                     | False, False =>
-                       fun _ _ => inl (exist _ False _)
-                     | True, _ =>
-                       fun _ _ => inl (exist _ True _)
-                     | _, True =>
-                       fun _ _ => inl (exist _ True _)
-                     | _, _ =>
-                       fun _ _ => inr (BoolEvalErr b)
-                     end eq_refl eq_refl
-                 | inr err, _ =>
-                   fun _ _ => inr err
-                 | _, inr err =>
-                   fun _ _ => inr err
-                 end eq_refl eq_refl
-             | Eq l r =>
-               fun _ =>
-                 match (sexp_step l Sigma pi) as lv', (sexp_step r Sigma pi) as rv'
-                       return (sexp_step l Sigma pi)=lv' ->
-                              (sexp_step r Sigma pi)=rv' ->
-                              (bool_value + error)
-                 with
-                 | inl (exist _ linner _),
-                   inl (exist _ rinner _) =>
-                   fun _ _ =>
-                     match linner as linner',
-                                     rinner as rinner'
-                           return linner=linner' ->
-                                  rinner=rinner' ->
-                                  (bool_value + error) with
-                     | (Cons ll lr), (Cons rl rr) =>
-                       fun _ _ =>
-                         bool_step (Conj (Eq ll rl) (Eq lr rr)) _
-                     | _, _ =>
-                       fun _ _ => inl (exist _ False _)
-                     end eq_refl eq_refl
-                 | inr err, _ =>
-                   fun _ _ => inr err
-                 | _, inr err =>
-                   fun _ _ => inr err
-                 end eq_refl eq_refl
-             | Mem l r =>
-               fun _ =>
-                 match (sexp_step l Sigma pi) as lv', (sexp_step r Sigma pi) as rv'
-                       return (sexp_step l Sigma pi)=lv' ->
-                              (sexp_step r Sigma pi)=rv' ->
-                              (bool_value + error)
-                 with
-                 | inl (exist _ linner _),
-                   inl (exist _ rinner _) =>
-                   fun _ _ =>
-                     match linner as linner', rinner as rinner'
-                           return linner = linner' ->
-                                  rinner = rinner' ->
-                                  (bool_value + error) with
-                     | lv, Cons rl rr =>
-                       fun _ _ =>
-                         bool_step (Disj (Eq lv rl) (Mem lv rr)) _
-                     | _, _ =>
-                       fun _ _ =>
-                         inl (exist _ False _)
-                     end eq_refl eq_refl
-                 | inr err, _ =>
-                   fun _ _ => inr err
-                 | _, inr err =>
-                   fun _ _ => inr err
-                 end eq_refl eq_refl
-             end eq_refl)) ; auto.
-  Unshelve.
-  * subst. intuition.
-    assert (sexp_is_value (Cons ll lr)). auto.
-    assert (sexp_is_value (Cons rl rr)). auto.
-    destruct l ; destruct r ; try discriminate.
-  - unfold sexp_step in e0 ; try discriminate.
-    assert (~sexp_is_value (Var n v)). unfold not. intros. inversion H1.
-      eapply t_trans with (Eq (Cons ll lr) (Cons rl rr)).
-      inversion s0. inversion s2.
-      + constructor. eapply EqLt ; auto.
-      + eapply t_trans with (Eq (Cons ll lr) (Var n0 v0)) ; constructor.
-        ** eapply SexpValueLtEqR; auto.
-           unfold not. intros. inversion H2.
-        ** eapply SexpValueLtEqL; auto.
-    - subst.
-      eapply t_trans with (Eq (Cons ll lr) (Cons rl rr)) ;
-      destruct (is_sexp_value (Cons r1 r2)).
-      + constructor.
-        inversion H. inversion H0.
-        eapply EqLt; auto.
-      + constructor.
-        inversion H. inversion H0.
-        eapply EqLt; auto.
-      + specialize canonical_sexp_value with (Cons r1 r2) Sigma pi s3.
-        intros.
-        rewrite H1 in e1.
-        assert ((Cons rl rr) = (Cons r1 r2)). injection e1. intros. crush.
-        constructor.
-        rewrite H2.
-        eapply SexpValueLtEqL; auto.
-        unfold not. intros. inversion H3.
-      + eapply t_trans with (Eq (Cons ll lr) (Cons r1 r2)).
-        ** constructor. eapply SexpValueLtEqR; auto.
-        **constructor. eapply SexpValueLtEqL; auto.
-          unfold not. intros. inversion H1.
-    - unfold sexp_step in e0 ; try discriminate.
-      fold sexp_step in e0.
-      eapply t_trans with (Eq (Cons ll lr) (Cons rl rr)) ;
-      destruct (is_sexp_value (Cons l1 l2)).
-      + constructor.
-        inversion H. inversion H0.
-        eapply EqLt; auto.
-      + constructor.
-        inversion H. inversion H0.
-        eapply EqLt; auto.
-      + specialize canonical_sexp_value with (Cons l1 l2) Sigma pi s3.
-        inversion s3.
-        specialize canonical_sexp_value with l1 Sigma pi H3.
-        specialize canonical_sexp_value with l2 Sigma pi H4.
-        intros.
-        destruct (sexp_step l1 Sigma pi).
-        ** destruct s6.
-           destruct (sexp_step l2 Sigma pi).
-           -- destruct s7.
-              subst.
-              assert ((Cons ll lr) = (Cons l1 l2)).
-              crush.
-              rewrite H1.
-              constructor.
-              eapply SexpValueLtEqR; auto.
-              unfold not. intros. inversion H2.
-           -- discriminate.
-              ** discriminate.
-      + eapply t_trans with (Eq (Cons l1 l2) (Cons rl rr)).
-        ** constructor. eapply SexpValueLtEqL; auto.
-        **constructor. eapply SexpValueLtEqR; auto.
-          unfold not. intros. inversion H1.
-    - inversion H. inversion H0. subst.
-      destruct (is_sexp_value (Cons l1 l2));
-        destruct (is_sexp_value (Cons r1 r2)).
-      + specialize canonical_sexp_value with (Cons l1 l2) Sigma pi s3.
-        specialize canonical_sexp_value with (Cons r1 r2) Sigma pi s4.
-        intros.
-        rewrite H2 in e0.
-        rewrite H1 in e1.
-        injection e0.
-        injection e1.
-        intros.
-        constructor.
-        rewrite H5.
-        rewrite H6.
-        rewrite H9.
-        rewrite H10.
-        eapply EqLt; auto.
-      + eapply t_trans with (Eq (Cons ll lr) (Cons rl rr)).
-        constructor. eapply EqLt; auto.
-        specialize canonical_sexp_value with (Cons l1 l2) Sigma pi s3.
-        intros.
-        rewrite H1 in e0.
-        injection e0.
-        intros.
-        rewrite H2. rewrite H5.
-        constructor.
-        eapply SexpValueLtEqR; auto.
-      + eapply t_trans with (Eq (Cons ll lr) (Cons rl rr)).
-        constructor. eapply EqLt; auto.
-        specialize canonical_sexp_value with (Cons r1 r2) Sigma pi s3.
-        intros.
-        rewrite H1 in e1.
-        injection e1.
-        intros.
-        rewrite H2. rewrite H5.
-        constructor.
-        eapply SexpValueLtEqL; auto.
-      + eapply t_trans with (Eq (Cons ll lr) (Cons rl rr)).
-        constructor. eapply EqLt; auto.
-        eapply t_trans with (Eq (Cons ll lr) (Cons r1 r2)).
-        constructor. eapply SexpValueLtEqR; auto.
-        constructor. eapply SexpValueLtEqL; auto.
-  * subst.
-    destruct (is_sexp_value l);
-      destruct (is_sexp_value r).
-    - specialize (@canonical_sexp_value_2 r (Cons rl rr) Sigma pi s2 s4 e1).
-      specialize (@canonical_sexp_value_2 l lv Sigma pi s0 s3 e0).
-      intros.
-      rewrite H, H0.
-      constructor.
-      inversion s2.
-      eapply MemLt; auto.
-    - eapply t_trans with (Mem lv (Cons rl rr)).
-      constructor.
-      inversion s2.
-      eapply MemLt; auto.
-      specialize (@canonical_sexp_value_2 l lv Sigma pi s0 s3 e0).
-      intros.
-      rewrite H.
-      constructor.
-      eapply SexpValueLtMemR; auto.
-    - specialize (@canonical_sexp_value_2 r (Cons rl rr) Sigma pi s2 s3 e1).
-      intros.
-      rewrite H.
-      eapply t_trans with (Mem lv (Cons rl rr)).
-      constructor.
-      inversion s2.
-      eapply MemLt; auto.
-      constructor.
-      eapply SexpValueLtMemL; auto.
-    - eapply t_trans with (Mem lv (Cons rl rr)).
-      constructor.
-      inversion s2.
-      eapply MemLt; auto.
-      eapply t_trans with (Mem l (Cons rl rr)).
-      constructor.
-      eapply SexpValueLtMemL; auto.
-      constructor.
-      eapply SexpValueLtMemR; auto.
-
-      * constructor.
-        subst.
-        solve [ eapply ConjLtR
-              | eapply DisjLtR
-              | eapply ConjLtL
-              | eapply DisjLtL
-              ].
-
-      * constructor.
-        subst.
-        solve [ eapply ConjLtR
-              | eapply DisjLtR
-              | eapply ConjLtL
-              | eapply DisjLtL
-              ].
-
-      * constructor.
-        subst.
-        solve [ eapply ConjLtR
-              | eapply DisjLtR
-              | eapply ConjLtL
-              | eapply DisjLtL
-              ].
-
-      * constructor.
-        subst.
-        solve [ eapply ConjLtR
-              | eapply DisjLtR
-              | eapply ConjLtL
-              | eapply DisjLtL
-              ].
-Qed.
-
-Definition merge_variable (Sig_o Sig_t: var_store_stack) (pi: principals) (mu: mergers) (key: node*var) (hval: sexp_value) (optsig: var_store + error)
-  : (var_store + error) :=
-  let (n, v) := key in
-  let orig_var := lookup n v Sig_o in
-  let curr_var := lookup n v Sig_t in
-  let sho := mu n v in
-  match optsig, orig_var, curr_var, sho with
-  | inl acc, inl oval, inl cval, Some sh =>
-    let hsig := set_env empty_env "scratch" "hypo" hval in
-    let osig := set_env hsig "scratch" "orig" oval in
-    let csig := set_env osig "scratch" "curr" cval in
-    match sexp_step sh (cons csig Sig_t) pi with
-    | inl val =>
-      inl (set_env acc n v val)
-    | inr err => inr err
-    end
-  | _, _, _, None => inr (MergeErr n v mu)
-  | inl acc, _, _, _ => inl acc
-  | inr err, _, _, _ => inr err
-  end.
-
-Fixpoint com_step (c: com) (sigma: var_store) (Sigma: var_store_stack) (omega: world_store) (pi: principals) (rho: location) (eta: handlers) (mu: mergers) : (var_store * world_store) + error :=
-  match c with
-  | Skip => inl (sigma, omega)
-  | Seq l r =>
-    match com_step l sigma Sigma omega pi rho eta mu with
-    | inl (sigma', omega') =>
-      com_step r sigma' Sigma omega' pi rho eta mu
-    | inr err => inr err
-    end
-  | If b t f =>
-    match bool_step (cons sigma Sigma) pi b as b' with
-    | inl (exist _ True _) => com_step t sigma Sigma omega pi rho eta mu
-    | inl (exist _ False _) => com_step f sigma Sigma omega pi rho eta mu
-    | inl _ => inr (BoolEvalErr b)
-    | inr err => inr err
-    end
-  | With n c' =>
-    com_step c' sigma Sigma omega (cons n pi) rho eta mu
-  | At n c' =>
-    com_step c' sigma Sigma omega pi n eta mu
-  | Handle n v op sh sm c' =>
-    let eta' := set_handler eta op n v sh in
-    let mu' := set_merger mu n v sm in
-    com_step c' sigma Sigma omega pi rho eta' mu'
-  | Op op =>
-    match eta op with
-    | Some (n, v, s) =>
-      match sexp_step s (cons sigma Sigma) pi with
-      | inl s' =>
-        match set_mem string_dec n pi with
-        | true =>
-          let sigma' := set_env sigma n v s' in
-          inl (sigma', omega)
-        | false => inr (WritePermErr n v pi)
+Fixpoint eval_sexp (s: sexp) (sigma: sigma_t) (omega: omega_t) (pi: pi_t) {struct s} : option sexp_value.
+  unshelve
+    refine (
+      match s with
+      | EmptySexp => Some (exist _ EmptySexp _)
+      | VarSexp n v =>
+        if pi_mem n pi then
+          sigma_get sigma n v
+        else
+          None
+      | WeightSexp w n v =>
+        match omega_get omega w with
+        | Some sigma_hyp =>
+          sigma_get sigma_hyp n v
+        | None =>
+          None
         end
-      | inr err => inr err
-      end
-    | None => inr (HandleErr op eta)
-    end
-  | Hyp w c =>
-    match com_step c empty_env (cons sigma Sigma) empty_world_store pi rho eta mu with
-    | inl (sigma', omega') =>
-      let omega'' := set_world_store omega w (cons sigma Sigma) sigma' in
-      inl (sigma, omega')
-    | inr err => inr err
-    end
-  | Commit w =>
-    match omega w with
-    | Some (Sigma_o, sigma_h) =>
-      let merge_fold := (merge_variable Sigma_o (cons sigma Sigma) (cons "scratch" pi) mu) in
-      match StringPairMap.fold merge_fold sigma_h (inl sigma) with
-      | inl sigma' => inl (sigma', omega)
-      | inr err => inr err
-      end
-    | None => inr (CommitErr w omega)
-    end
-  end.
+      | ConsSexp s1 s2 =>
+        match eval_sexp s1 sigma omega pi,
+              eval_sexp s2 sigma omega pi with
+        | Some (exist _ s1v _), Some (exist _ s2v _) =>
+          Some (exist _ (ConsSexp s1v s2v) _)
+        | _, _ => None
+        end
+      end)
+  .
+  constructor.
+  constructor ; auto.
+Defined.
 
-Definition run (c: com) :=
-  match com_step c empty_env nil empty_world_store nil "" empty_handlers empty_mergers with
-  | inl (sigma, omega) => inl sigma
-  | inr err => inr err
-  end.
 
-Definition test_com := (Seq (With "alice" (Handle "alice" "times" "__tmp" (Cons EmptySet (Cons EmptySet (Cons EmptySet (Cons EmptySet EmptySet)))) EmptySet (Op "__tmp"))) (Seq (With "bob" (Handle "bob" "times" "__tmp" (Cons EmptySet (Cons EmptySet (Cons EmptySet (Cons EmptySet EmptySet)))) EmptySet (Op "__tmp"))) (With "alice" (Seq (Handle "alice" "fitness" "__tmp" EmptySet EmptySet (Op "__tmp")) (Seq (Handle "alice" "fitness" "set_fitness" (Cons (Var "alice" "fitness") (Var "bob" "fitness")) (Cons (Var "scratch" "orig") (Cons (Var "scratch" "hypo") (Var "scratch" "curr"))) (Hyp "world" (At "DataCenter" (With "Bob" (Op "set_fitness"))))) (Commit "world")))))).
+Fixpoint eval_bool (b: bool) (sigma: sigma_t) (omega: omega_t) (pi: pi_t) {struct b} : option bool_value.
+  unshelve
+    refine (
+      match b with
+      | TrueBool => Some (exist _ TrueBool _)
+      | FalseBool => Some (exist _ FalseBool _)
+      | ConjBool b1 b2 =>
+        match eval_bool b1 sigma omega pi,
+              eval_bool b2 sigma omega pi
+        with
+        | Some (exist _ TrueBool _), Some b2' => Some b2'
+        | Some (exist _ FalseBool _), Some b2' => Some (exist _ FalseBool _)
+        | _, _ => None
+        end
+      | DisjBool b1 b2 =>
+        match eval_bool b1 sigma omega pi,
+              eval_bool b2 sigma omega pi
+        with
+        | Some (exist _ FalseBool _), Some b2' => Some b2'
+        | Some (exist _ TrueBool _), Some b2' => Some (exist _ TrueBool _)
+        | _, _ => None
+        end
+      | EqBool s1 s2 =>
+        match eval_sexp s1 sigma omega pi,
+              eval_sexp s2 sigma omega pi
+        with
+        | Some (exist _ l lp), Some (exist _ r rp) => Some (eval_eq l r lp rp)
+        | _, _ => None
+        end
+      | MemBool s1 s2 =>
+        match eval_sexp s1 sigma omega pi,
+              eval_sexp s2 sigma omega pi
+        with
+        | Some (exist _ l lp), Some (exist _ r rp) => Some (eval_mem l r lp rp)
+        | _, _ => None
+        end
+      end)
+  ;
+  eauto.
+Defined.
 
-Eval native_compute in (run test_com).
+Fixpoint eval_com (c: com) (sigma: sigma_t) (omega: omega_t) (pi: pi_t) (rho: rho_t) (mu: mu_t) {struct c} : option (sigma_t * omega_t).
+  unshelve (
+      refine (
+          match c with
+          | SkipCom => Some (sigma, omega)
+          | SeqCom c1 c2 =>
+            match eval_com c1 sigma omega pi rho mu with
+            | None => None
+            | Some (sigma', omega') =>
+              eval_com c2 sigma' omega' pi rho mu
+            end
+          | IfCom b c1 c2 =>
+            match eval_bool b sigma omega pi with
+            | Some (exist _ TrueBool _) =>
+              eval_com c1 sigma omega pi rho mu
+            | Some (exist _ FalseBool _) =>
+              eval_com c2 sigma omega pi rho mu
+            | _ => None
+            end
+          | WithCom n c =>
+            eval_com c sigma omega (pi_add n pi) rho mu
+          | AtCom n c =>
+            eval_com c sigma omega pi n mu
+          | WorldAssignCom u c =>
+            match eval_com c sigma omega_0 pi rho mu with
+            | None => None
+            | Some (sigma_hyp, omega_hyp) =>
+              Some (sigma, omega_set omega u sigma_hyp)
+            end
+          | CommitCom w =>
+            match omega_get omega w with
+            | None => None
+            | Some sigma_hyp =>
+              let merged_sigma : NodeVarMap.t (option sexp_value) :=
+                  NodeVarMap.mapi
+                    (fun key sh =>
+                       match key with
+                       | (n, v) =>
+                         match mu_get mu n v,
+                               sigma_get sigma n v
+                         with
+                         | Some merge_func, Some sc =>
+                           Some (merge_func sc sh)
+                         | _, _ => None
+                         end
+                       end)
+                    sigma_hyp
+              in
+              match
+                NodeVarMap.fold
+                  (fun k vo so =>
+                     match vo, so with
+                     | Some v, Some s =>
+                       Some (NodeVarMap.add k v s)
+                     | _, _ => None
+                     end) merged_sigma (Some sigma)
+              with
+              | None => None
+              | Some sigma' =>
+                Some (sigma', omega)
+              end
+            end
+          end
+        )
+    ).
+Defined.
