src/OpalProofs.v
@@ -1,0 +1,295 @@
+Require Import Opal.OpalSemantics CpdtTactics.
+
+Definition omega_reps (omega: omega_t) (Omega: Omega_t) : Prop :=
+  forall k, Omega_in Omega k -> (exists v, WorldVarMap.MapsTo k v omega).
+
+Definition sigma_reps (sigma: sigma_t) (Sigma: Sigma_t) : Prop :=
+  forall n v, Sigma_in Sigma n v ->
+              exists val, sigma_get sigma n v = Some val.
+
+Theorem sexp_progress:
+  forall s omega sigma Omega Pi Sigma,
+    well_formed_sexp s Omega Pi Sigma ->
+    omega_reps omega Omega ->
+    sigma_reps sigma Sigma ->
+    (exists sv, eval_sexp s sigma omega Pi = Some sv).
+Proof.
+  induction s ; intros ; inversion H ; subst.
+  * unfold eval_sexp. eauto.
+  * assert (pi_mem n Pi = true).
+    unfold Pi_in in H8. unfold pi_mem.
+    eapply NodeMap.mem_1.
+    unfold NodeMap.In. exists tt. auto.
+    unfold sigma_reps in H1.
+    specialize (H1 n v H8).
+    inversion H1.
+    exists x.
+    unfold eval_sexp.
+    rewrite H2.
+    apply H3.
+  * assert (pi_mem n Pi = true).
+    eapply NodeMap.mem_1.
+    unfold NodeMap.In. exists tt. auto.
+
+    unfold eval_sexp.
+    unfold omega_reps in H0.
+    specialize (H0 w).
+    intuition.
+    destruct H3.
+    specialize (WorldVarMap.find_1 H0).
+    intros.
+    unfold omega_get.
+    rewrite H3.
+
+    unfold sigma_reps in H1.
+    specialize (H1 n v).
+    intuition.
+    destruct H4.
+    exists x0.
+    eauto.
+
+    unfold omega_reps in H0.
+    specialize (H0 w).
+    intuition.
+    unfold omega_get.
+    inversion H3.
+    specialize (WorldVarMap.find_1 H0).
+    edestruct WorldVarMap.find ; intros ; try discriminate.
+    injection H4 ; clear H4.
+    intros. subst.
+    unfold eval_sexp.
+    destruct H3.
+    unfold omega_get.
+    specialize (WorldVarMap.find_1 H0). intros. rewrite H4.
+    destruct (sigma_get x n v) eqn:? ; eauto.
+  * specialize (IHs1 omega sigma Omega Sigma Pi).
+    specialize (IHs2 omega sigma Omega Sigma Pi).
+    intuition.
+    inversion H2. inversion H3.
+    unfold eval_sexp.
+    fold eval_sexp.
+    edestruct eval_sexp; edestruct eval_sexp; eauto.
+Qed.
+
+Theorem bool_progress:
+  forall b omega sigma Omega Sigma Pi,
+    well_formed_bool b Omega Sigma Pi ->
+    omega_reps omega Omega ->
+    sigmas_reps sigma Sigma ->
+    (exists bv, eval_bool b sigma omega Pi = Some bv).
+Proof.
+  induction b ; intros ; inversion H ; subst.
+  * unfold eval_bool. eauto.
+  * unfold eval_bool. eauto.
+  * specialize (IHb1 omega sigma Omega Sigma Pi H4 H0 H1).
+    specialize (IHb2 omega sigma Omega Sigma Pi H8 H0 H1).
+    crush.
+    destruct x0 ; eauto.
+  * specialize (IHb1 omega sigma Omega Sigma Pi H4 H0 H1).
+    specialize (IHb2 omega sigma Omega Sigma Pi H8 H0 H1).
+    crush.
+    destruct x0 ; eauto.
+  * specialize (sexp_progress) as sp1.
+    specialize (sexp_progress) as sp2.
+    specialize (sp1 s omega sigma Omega Sigma Pi H4 H0 H1).
+    specialize (sp2 s0 omega sigma Omega Sigma Pi H8 H0 H1).
+    crush.
+    eauto.
+  * specialize (sexp_progress) as sp1.
+    specialize (sexp_progress) as sp2.
+    specialize (sp1 s omega sigma Omega Sigma Pi H4 H0 H1).
+    specialize (sp2 s0 omega sigma Omega Sigma Pi H8 H0 H1).
+    crush.
+    eauto.
+Qed.
+
+
+Theorem progress:
+  forall c sigmas Sigma omega Omega Pi eta Eta mu rho,
+    sigmas <> nil ->
+    omega_reps omega Omega ->
+    sigmas_reps sigmas Sigma ->
+    eta_reps eta Eta ->
+    mu_reps mu Sigma ->
+    (exists Omega', well_formed_com c Omega Sigma Pi Eta Omega') ->
+    exists sigma' omega',
+      eval_com c sigmas omega Pi rho eta mu = Some (sigma', omega').
+Proof.
+  induction c ; intros ; unfold eval_com ; fold eval_com.
+  * intros. destruct sigmas. contradiction H. reflexivity.
+    exists s. exists omega. auto.
+  * inversion H4.
+    inversion H5.
+  * inversion H4. inversion H5.
+    subst. intuition.
+
+    specialize (bool_progress).
+    intros.
+
+    destruct sigmas. contradiction H. reflexivity.
+    specialize (H6 b omega (s::sigmas) Omega Sigma Pi H10 H0 H1).
+    destruct (eval_bool b (s :: sigmas) omega Pi).
+    specialize (IHc1 (s::sigmas) Sigma omega Omega Pi eta Eta mu rho).
+    specialize (IHc2 (s::sigmas) Sigma omega Omega Pi eta Eta mu rho).
+    destruct b0.
+  - intuition.
+    eapply H9.
+    exists Omega'.
+    auto.
+  - intuition.
+    eapply H7.
+    exists Omega''.
+    auto.
+  - inversion H6. inversion H7.
+    * destruct sigmas. contradiction H. reflexivity.
+      specialize (IHc (s::sigmas) Sigma omega Omega (pi_add n Pi) eta Eta mu rho).
+      intuition.
+      assert (exists Omega' : Omega_t,
+                 well_formed_com c Omega Sigma (pi_add n Pi) Eta Omega').
+  - inversion H4. inversion H6. subst. exists x. apply H15.
+  - crush.
+    * destruct sigmas. contradiction H. reflexivity.
+      specialize (IHc (s::sigmas) Sigma omega Omega Pi eta Eta mu n).
+      intuition.
+      assert (exists Omega' : Omega_t, well_formed_com c Omega Sigma Pi Eta Omega').
+  - destruct H4. exists x. inversion H4. auto.
+  - intuition.
+    * destruct sigmas. contradiction H. reflexivity.
+      inversion H4.
+      inversion H5.
+      assert (pi_mem n Pi = true). specialize (NodeSet.mem_spec Pi n). crush.
+      subst.
+      rewrite H26.
+      remember (sigma_set s1 n v EmptySexpValue) as s2.
+      pose (OpSet.add o Eta).
+      pose (NodeVarSet.add (n,v) Sigma).
+      specialize (IHc (s2::sigmas) (NodeVarSet.add (n, v) Sigma) omega Omega Pi (eta_set eta o n v s) t (mu_set mu n v v0 v1 v2 s0) n).
+      intuition.
+
+      assert (s2 :: sigmas = nil -> False).
+      intros. discriminate.
+
+      assert (sigmas_reps (s2 :: sigmas) (NodeVarSet.add (n, v) Sigma)).
+      unfold sigmas_reps in *.
+      unfold sigmas_get in *.
+      unfold sigma_set in *.
+      intros.
+      destruct (NodeVarType.eq_dec (n,v) (n0,v3)).
+  - specialize (NodeVarMap.add_1 s1 EmptySexpValue e).
+    intros.
+    exists (EmptySexpValue).
+    specialize (NodeVarMap.find_1 H8).
+    intros.
+    rewrite <- Heqs2 in H9.
+    assert (sigma_get s2 n0 v3 = Some EmptySexpValue).
+    + crush.
+    + rewrite H10. auto.
+  - fold sigmas_get in *.
+    specialize (H1 n0 v3).
+    specialize (NodeVarSet.add_spec Sigma (n,v) (n0,v3)).
+    intros.
+    destruct H8.
+    intuition.
+    destruct (sigma_get s2 n0 v3) eqn:?.
+    + exists s3. auto.
+    + inversion H10.
+      destruct (sigma_get s1 n0 v3) eqn:?.
+      ** subst.
+         unfold sigma_get in *.
+         specialize (NodeVarMap.find_2 Heqo1).
+         intros.
+         specialize (NodeVarMap.add_2 EmptySexpValue n1 H13).
+         intros.
+         specialize (NodeVarMap.find_1 H14).
+         intros.
+         assert (sigma_get (NodeVarMap.add (n, v) EmptySexpValue s1) n0 v3 = Some s3). unfold sigma_get. auto.
+         assert (sigma_get (NodeVarMap.add (n, v) EmptySexpValue s1) n0 v3 = None). unfold sigma_get. auto.
+         rewrite H16 in H17. discriminate.
+      ** auto.
+  -
+    assert (eta_reps (eta_set eta o n v s) t).
+    unfold eta_reps in *.
+    intros.
+    unfold eta_get in *.
+    unfold eta_set in *.
+    destruct (OpType.eq_dec o op0).
+    specialize (OpMap.add_1 eta (n,v,s) e).
+    exists (n,v,s).
+    specialize (OpMap.find_1 H9).
+    intros.
+    auto.
+    subst.
+    specialize H2 with op0.
+    assert (OpSet.In op0 Eta).
+    specialize (OpSet.add_spec Eta o op0).
+    intuition.
+    intuition.
+    inversion H11.
+    exists x0.
+    specialize (OpMap.find_2 H2).
+    intros.
+    specialize (OpMap.add_2 (n,v,s) n0 H12).
+    intros.
+    specialize (OpMap.find_1 H13).
+    auto.
+
+    assert (mu_reps (mu_set mu n v v0 v1 v2 s0) (NodeVarSet.add (n, v) Sigma)).
+    unfold mu_reps in *.
+    unfold mu_get in *.
+    unfold mu_set in *.
+    intros.
+    destruct (NodeVarType.eq_dec (n,v) (n0,v3)) eqn:?.
+    + specialize (NodeVarMap.add_1 mu (v0, v1, v2, s0) e).
+      intros.
+      specialize (NodeVarMap.find_1 H10).
+      intros.
+      exists (v0,v1,v2,s0). auto.
+    + specialize (H3 n0 v3).
+      assert (NodeVarSet.In (n0, v3) Sigma).
+      specialize (NodeVarSet.add_spec Sigma (n,v) (n0,v3)).
+      intros.
+      destruct H10. intuition.
+      intuition.
+      inversion H11.
+      specialize (NodeVarMap.find_2 H3).
+      intros.
+      specialize (NodeVarMap.add_2 (v0, v1, v2, s0) n1 H13).
+      intros.
+      exists x0.
+      specialize (NodeVarMap.find_1 H14).
+      intros.
+      auto.
+    + assert (exists Omega', well_formed_com c Omega (NodeVarSet.add (n, v) Sigma) Pi t Omega').
+      exists x. auto.
+
+      intuition.
+      * destruct sigmas. contradiction H. reflexivity.
+        inversion H4.
+        inversion H5.
+        subst.
+        unfold eta_reps in *.
+        unfold eta_get in *.
+        specialize (H2 o H8).
+        inversion H2.
+        rewrite H6.
+        destruct x0, p.
+        pose
+
+          subst. intuition.
+        specialize (IHc n Pi).
+        eapply IHc.
+        eauto.
+      * inversion H. inversion H0.
+        subst. intuition.
+        specialize (IHc n Pi).
+        assert (pi_mem n Pi = true). inversion H16.
+        crush.
+  - inversion H16; subst.
+    +
+
+      specialize (NodeSet.mem_spec Pi n). crush.
+      assert
+        inversion H16.
+      crush.
+      eapply IHc.
+Qed.
